src/Classes.v
@@ -194,6 +194,7 @@ Global Instance ArbitraryOfGenShrink {A} `{Gen A} `{Shrink A} : Arbitrary A.
 
 Generalizable Variables PSized PMon PSMon PCorr.
 
+(*
 Instance GenMonotonicOfSized (A : Type)
          {H : GenSized A}
          `{@GenSizedMonotonic A H PMon}
@@ -214,6 +215,7 @@ Proof.
     split. intros [n H3]. constructor; eauto.
     intros H4. eexists; split; eauto.
 Qed.
+*)
 
 Lemma nat_set_ind (A : Type) `{GenSized A} `{Hyp : CanonicalSized A} :
   (semGen (arbitrarySized 0) <--> zeroSized) ->
